Remove _ from mem_inj for consistency's sake.

refinements.v
@@ -2,41 +2,41 @@
 (* This file is distributed under the terms of the BSD license. *)
 Require Export references memory_basics.
 
-Inductive mem_inj (Ti : Set) :=
-  | mem_inj_id : mem_inj Ti
-  | mem_inj_map : indexmap (index * ref Ti) → mem_inj Ti.
-Arguments mem_inj_id {_}.
-Arguments mem_inj_map {_} _.
-Instance mem_inj_dec {Ti : Set} `{∀ τi1 τi2 : Ti, Decision (τi1 = τi2)}
-  (f g : mem_inj Ti) : Decision (f = g).
+Inductive meminj (Ti : Set) :=
+  | meminj_id : meminj Ti
+  | meminj_map : indexmap (index * ref Ti) → meminj Ti.
+Arguments meminj_id {_}.
+Arguments meminj_map {_} _.
+Instance meminj_dec {Ti : Set} `{∀ τi1 τi2 : Ti, Decision (τi1 = τi2)}
+  (f g : meminj Ti) : Decision (f = g).
 Proof. solve_decision. Defined.
-Instance mem_inj_lookup {Ti} : Lookup index (index * ref Ti) (mem_inj Ti) :=
-  λ o f, match f with mem_inj_id => Some (o, []) | mem_inj_map m => m !! o end.
-Definition mem_inj_compose {Ti} (f g : mem_inj Ti) : mem_inj Ti :=
+Instance meminj_lookup {Ti} : Lookup index (index * ref Ti) (meminj Ti) :=
+  λ o f, match f with meminj_id => Some (o, []) | meminj_map m => m !! o end.
+Definition meminj_compose {Ti} (f g : meminj Ti) : meminj Ti :=
   match f, g with
-  | mem_inj_id, mem_inj_id => mem_inj_id
-  | mem_inj_map m, mem_inj_id => mem_inj_map m
-  | mem_inj_id, mem_inj_map m => mem_inj_map m
-  | mem_inj_map m1, mem_inj_map m2 => mem_inj_map $
+  | meminj_id, meminj_id => meminj_id
+  | meminj_map m, meminj_id => meminj_map m
+  | meminj_id, meminj_map m => meminj_map m
+  | meminj_map m1, meminj_map m2 => meminj_map $
      merge (λ yr _ : option (index * ref Ti),
        '(y1,r1) ← yr; '(y2,r2) ← m2 !! y1; Some (y2, r1 ++ r2)) m1 ∅
   end.
-Arguments mem_inj_compose _ !_ !_ /.
-Infix "◎" := mem_inj_compose (at level 40, left associativity) : C_scope.
-Notation "(◎)" := mem_inj_compose (only parsing) : C_scope.
+Arguments meminj_compose _ !_ !_ /.
+Infix "◎" := meminj_compose (at level 40, left associativity) : C_scope.
+Notation "(◎)" := meminj_compose (only parsing) : C_scope.
 
-Definition mem_inj_injective {Ti} (f : mem_inj Ti) : Prop := ∀ o1 o2 o r1 r2,
+Definition meminj_injective {Ti} (f : meminj Ti) : Prop := ∀ o1 o2 o r1 r2,
   f !! o1 = Some (o,r1) → f !! o2 = Some (o,r2) → o1 = o2 ∨ r1 ⊥ r2.
-Instance mem_inj_subseteq {Ti} : SubsetEq (mem_inj Ti) := λ f1 f2,
+Instance meminj_subseteq {Ti} : SubsetEq (meminj Ti) := λ f1 f2,
   ∀ o o' r', f1 !! o = Some (o',r') → f2 !! o = Some (o',r').
 
-Section mem_inj.
+Section meminj.
 Context {Ti : Set}.
-Implicit Types f g : mem_inj Ti.
+Implicit Types f g : meminj Ti.
 Implicit Types o : index.
 Implicit Types r : ref Ti.
 
-Lemma mem_inj_eq f g : (∀ o, f !! o = g !! o) → f = g.
+Lemma meminj_eq f g : (∀ o, f !! o = g !! o) → f = g.
 Proof.
   intros Hfg. destruct f as [|m1], g as [|m2].
   * done.
@@ -47,12 +47,12 @@ Proof.
   * f_equal. apply map_eq, Hfg.
 Qed.
 
-Lemma lookup_mem_inj_id o : @mem_inj_id Ti !! o = Some (o, []).
+Lemma lookup_meminj_id o : @meminj_id Ti !! o = Some (o, []).
 Proof. done. Qed.
-Lemma lookup_mem_inj_id_Some o1 o2 r :
-  mem_inj_id !! o1 = Some (o2,r) ↔ o2 = o1 ∧ r = [].
+Lemma lookup_meminj_id_Some o1 o2 r :
+  meminj_id !! o1 = Some (o2,r) ↔ o2 = o1 ∧ r = [].
 Proof. naive_solver. Qed.
-Lemma lookup_mem_inj_compose f g o :
+Lemma lookup_meminj_compose f g o :
   (f ◎ g) !! o = '(y1,r1) ← f !! o; '(y2,r2) ← g !! y1; Some (y2,r1 ++ r2).
 Proof.
   unfold lookup; destruct f as [|m1], g as [|m2]; csimpl.
@@ -61,39 +61,39 @@ Proof.
   * by destruct (_ !! o) as [[??]|]; csimpl; rewrite ?(right_id_L [] (++)).
   * by rewrite lookup_merge by done.
 Qed.
-Lemma lookup_mem_inj_compose_Some f g o1 o3 r :
+Lemma lookup_meminj_compose_Some f g o1 o3 r :
   (f ◎ g) !! o1 = Some (o3,r) ↔
   ∃ o2 r2 r3, f !! o1 = Some (o2,r2) ∧ g !! o2 = Some (o3,r3) ∧ r = r2 ++ r3.
 Proof.
-  rewrite lookup_mem_inj_compose. split.
+  rewrite lookup_meminj_compose. split.
   * intros. destruct (f !! o1) as [[o2 r2]|] eqn:?; simplify_equality'.
     destruct (g !! o2) as [[??]|] eqn:?; naive_solver.
   * by intros (?&?&?&?&?&?); simplify_option_equality.
 Qed.
 
-Global Instance: LeftId (@eq (mem_inj Ti)) mem_inj_id (◎).
+Global Instance: LeftId (@eq (meminj Ti)) meminj_id (◎).
 Proof. by intros []. Qed.
-Global Instance: RightId (@eq (mem_inj Ti)) mem_inj_id (◎).
+Global Instance: RightId (@eq (meminj Ti)) meminj_id (◎).
 Proof. by intros []. Qed.
-Global Instance: Associative (@eq (mem_inj Ti)) (◎).
+Global Instance: Associative (@eq (meminj Ti)) (◎).
 Proof.
-  intros f g h. apply mem_inj_eq. intros o1. rewrite !lookup_mem_inj_compose.
+  intros f g h. apply meminj_eq. intros o1. rewrite !lookup_meminj_compose.
   destruct (f !! o1) as [[o2 r2]|]; csimpl; [|done].
-  rewrite !lookup_mem_inj_compose.
+  rewrite !lookup_meminj_compose.
   destruct (g !! o2) as [[o3 r3]|]; csimpl; [|done].
   by destruct (h !! o3) as [[??]|]; csimpl; rewrite ?(associative_L (++)).
 Qed.
-Lemma mem_inj_positive_l f g : f ◎ g = mem_inj_id → f = mem_inj_id.
+Lemma meminj_positive_l f g : f ◎ g = meminj_id → f = meminj_id.
 Proof. by destruct f, g. Qed.
-Lemma mem_inj_positive_r f g : f ◎ g = mem_inj_id → g = mem_inj_id.
+Lemma meminj_positive_r f g : f ◎ g = meminj_id → g = meminj_id.
 Proof. by destruct f, g. Qed.
 
-Lemma mem_inj_id_injective : mem_inj_injective (@mem_inj_id Ti).
+Lemma meminj_id_injective : meminj_injective (@meminj_id Ti).
 Proof. intros x1 x2 y r1 r2 ??; simplify_equality'; auto. Qed.
-Lemma mem_inj_compose_injective f g :
-  mem_inj_injective f → mem_inj_injective g → mem_inj_injective (f ◎ g).
+Lemma meminj_compose_injective f g :
+  meminj_injective f → meminj_injective g → meminj_injective (f ◎ g).
 Proof.
-  intros Hf Hg o1 o2 o r1 r2; rewrite !lookup_mem_inj_compose_Some.
+  intros Hf Hg o1 o2 o r1 r2; rewrite !lookup_meminj_compose_Some.
   intros (o1'&r1'&r1''&?&?&->) (o2'&r2'&r2''&?&?&->).
   destruct (decide (o1 = o2)); [by left|].
   destruct (Hg o1' o2' o r1'' r2'') as [->|?]; simplify_equality'; auto.
@@ -101,38 +101,38 @@ Proof.
     right. by apply ref_disjoint_here_app_1. }
   right. by apply ref_disjoint_app_l, ref_disjoint_app_r.
 Qed.
-Lemma mem_inj_injective_alt f o1 o2 o r1 r2 :
-  mem_inj_injective f → f !! o1 = Some (o,r1) → f !! o2 = Some (o,r2) →
+Lemma meminj_injective_alt f o1 o2 o r1 r2 :
+  meminj_injective f → f !! o1 = Some (o,r1) → f !! o2 = Some (o,r2) →
   o1 = o2 ∨ o1 ≠ o2 ∧ r1 ⊥ r2.
 Proof.
   intros Hf ??. destruct (decide (o1 = o2)); [by left|].
   destruct (Hf o1 o2 o r1 r2); auto.
 Qed.
-Lemma mem_inj_injective_ne f o1 o2 o3 o4 r2 r4 :
-  mem_inj_injective f → f !! o1 = Some (o2,r2) → f !! o3 = Some (o4,r4) →
+Lemma meminj_injective_ne f o1 o2 o3 o4 r2 r4 :
+  meminj_injective f → f !! o1 = Some (o2,r2) → f !! o3 = Some (o4,r4) →
   o1 ≠ o3 → o2 ≠ o4 ∨ o2 = o4 ∧ r2 ⊥ r4.
 Proof.
   intros Hf ???. destruct (decide (o2 = o4)) as [->|]; auto.
   destruct (Hf o1 o3 o4 r2 r4); auto.
 Qed.
-Global Instance: PartialOrder ((⊆) : relation (mem_inj Ti)).
+Global Instance: PartialOrder ((⊆) : relation (meminj Ti)).
 Proof.
   repeat split.
   * by intros f o o' r'.
-  * intros f1 f2 f3. unfold subseteq, mem_inj_subseteq. naive_solver.
-  * intros f1 f2; unfold subseteq, mem_inj_subseteq; intros.
-    apply mem_inj_eq. intros o. apply option_eq. intros [o' r']; naive_solver.
+  * intros f1 f2 f3. unfold subseteq, meminj_subseteq. naive_solver.
+  * intros f1 f2; unfold subseteq, meminj_subseteq; intros.
+    apply meminj_eq. intros o. apply option_eq. intros [o' r']; naive_solver.
 Qed.
-End mem_inj.
+End meminj.
 
-Class RefineM Ti E A := refineM: E → mem_inj Ti → relation A.
+Class RefineM Ti E A := refineM: E → meminj Ti → relation A.
 Class Refine Ti E A :=
-  refine: E → mem_inj Ti → memenv Ti → memenv Ti → A → A → Prop.
-Class RefineTM Ti E T A := refineTM: E → mem_inj Ti → A → A → T → Prop.
+  refine: E → meminj Ti → memenv Ti → memenv Ti → A → A → Prop.
+Class RefineTM Ti E T A := refineTM: E → meminj Ti → A → A → T → Prop.
 Class RefineT Ti E T A :=
-  refineT: E → mem_inj Ti → memenv Ti → memenv Ti → A → A → T → Prop.
+  refineT: E → meminj Ti → memenv Ti → memenv Ti → A → A → T → Prop.
 Class PathRefine Ti E T1 T2 A :=
-  path_refine: E → mem_inj Ti → memenv Ti → memenv Ti → A → A → T1 → T2 → Prop.
+  path_refine: E → meminj Ti → memenv Ti → memenv Ti → A → A → T1 → T2 → Prop.
 Instance: Params (@refineM) 4.
 Instance: Params (@refine) 4.
 Instance: Params (@refineTM) 5.
@@ -141,13 +141,13 @@ Instance: Params (@path_refine) 6.
 
 Notation "X ⊑{ Γ , f } Y" := (refineM Γ f X Y)
   (at level 70, format "X  ⊑{ Γ , f }  Y") : C_scope.
-Notation "X ⊑{ Γ } Y" := (X ⊑{Γ,mem_inj_id} Y)
+Notation "X ⊑{ Γ } Y" := (X ⊑{Γ,meminj_id} Y)
   (at level 70, format "X  ⊑{ Γ }  Y") : C_scope.
 
 Notation "X ⊑{ Γ , f } Y : τ" := (refineTM Γ f X Y τ)
   (at level 70, Y at next level,
    format "X  ⊑{ Γ , f }  Y  :  τ") : C_scope.
-Notation "X ⊑{ Γ } Y : τ" := (X ⊑{Γ,mem_inj_id} Y : τ)
+Notation "X ⊑{ Γ } Y : τ" := (X ⊑{Γ,meminj_id} Y : τ)
   (at level 70, Y at next level, format "X  ⊑{ Γ }  Y  :  τ") : C_scope.
 
 Notation "X ⊑{ Γ , f @ m1 ↦ m2 } Y" := (refine Γ f m1 m2 X Y)
@@ -157,11 +157,11 @@ Notation "Xs ⊑{ Γ , f @ m1 ↦ m2 }* Ys" := (Forall2 (refine Γ f m1 m2) Xs Y
 Notation "Xss ⊑{ Γ , f @ m1 ↦ m2 }2** Yss" :=
   (Forall2 (λ Xs Ys, Xs.2 ⊑{Γ,f @ m1↦m2}* Ys.2) Xss Yss)
   (at level 70, format "Xss  ⊑{ Γ , f  @  m1 ↦ m2 }2**  Yss") : C_scope.
-Notation "X ⊑{ Γ @ m } Y" := (X ⊑{Γ,mem_inj_id @ m↦m} Y)
+Notation "X ⊑{ Γ @ m } Y" := (X ⊑{Γ,meminj_id @ m↦m} Y)
   (at level 70, format "X  ⊑{ Γ  @  m }  Y") : C_scope.
-Notation "Xs ⊑{ Γ @ m }* Ys" := (Xs ⊑{Γ,mem_inj_id @ m↦m}* Ys)
+Notation "Xs ⊑{ Γ @ m }* Ys" := (Xs ⊑{Γ,meminj_id @ m↦m}* Ys)
   (at level 70, format "Xs  ⊑{ Γ  @  m }*  Ys") : C_scope.
-Notation "Xss ⊑{ Γ @ m }2** Yss" := (Xss ⊑{Γ,mem_inj_id @ m↦m}2** Yss)
+Notation "Xss ⊑{ Γ @ m }2** Yss" := (Xss ⊑{Γ,meminj_id @ m↦m}2** Yss)
   (at level 70, format "Xss  ⊑{ Γ  @  m }2**  Yss") : C_scope.
 
 Notation "X ⊑{ Γ , f @ m1 ↦ m2 } Y : τ" := (refineT Γ f m1 m2 X Y τ)
@@ -179,23 +179,23 @@ Notation "Xs ⊑{ Γ , f @ m1 ↦ m2 }1* Ys :* τs" :=
   (Forall3 (λ X Y τ, X.1 ⊑{Γ,f @ m1↦m2} Y.1 : τ) Xs Ys τs)
   (at level 70, Ys at next level,
    format "Xs  ⊑{ Γ , f  @  m1 ↦ m2 }1*  Ys  :*  τs") : C_scope.
-Notation "X ⊑{ Γ @ m } Y : τ" := (X ⊑{Γ,mem_inj_id @ m↦m} Y : τ)
+Notation "X ⊑{ Γ @ m } Y : τ" := (X ⊑{Γ,meminj_id @ m↦m} Y : τ)
   (at level 70, Y at next level,
    format "X  ⊑{ Γ  @  m }  Y  :  τ") : C_scope.
-Notation "Xs ⊑{ Γ @ m }* Ys : τ" := (Xs ⊑{Γ,mem_inj_id @ m↦m}* Ys : τ)
+Notation "Xs ⊑{ Γ @ m }* Ys : τ" := (Xs ⊑{Γ,meminj_id @ m↦m}* Ys : τ)
   (at level 70, Ys at next level,
    format "Xs  ⊑{ Γ  @  m }*  Ys  :  τ") : C_scope.
-Notation "Xs ⊑{ Γ @ m }* Ys :* τs" := (Xs ⊑{Γ,mem_inj_id @ m↦m}* Ys :* τs)
+Notation "Xs ⊑{ Γ @ m }* Ys :* τs" := (Xs ⊑{Γ,meminj_id @ m↦m}* Ys :* τs)
   (at level 70, Ys at next level,
    format "Xs  ⊑{ Γ  @  m }*  Ys  :*  τs") : C_scope.
-Notation "Xs ⊑{ Γ @ m }1* Ys :* τs" := (Xs ⊑{Γ,mem_inj_id @ m↦m}1* Ys :* τs)
+Notation "Xs ⊑{ Γ @ m }1* Ys :* τs" := (Xs ⊑{Γ,meminj_id @ m↦m}1* Ys :* τs)
   (at level 70, Ys at next level,
    format "Xs  ⊑{ Γ  @  m }1*  Ys  :*  τs") : C_scope.
 
 Notation "X ⊑{ Γ , f @ m1 ↦ m2 } Y : τ ↣ σ" := (path_refine Γ f m1 m2 X Y τ σ)
   (at level 70, Y at next level, τ at next level, σ at next level,
    format "X  ⊑{ Γ , f  @  m1 ↦ m2 }  Y  :  τ  ↣  σ") : C_scope.
-Notation "X ⊑{ Γ @ m } Y : τ ↣ σ" := (X ⊑{ Γ , mem_inj_id @ m ↦ m } Y : τ ↣ σ)
+Notation "X ⊑{ Γ @ m } Y : τ ↣ σ" := (X ⊑{ Γ , meminj_id @ m ↦ m } Y : τ ↣ σ)
   (at level 70, Y at next level, τ at next level, σ at next level,
    format "X  ⊑{ Γ  @  m }  Y  :  τ  ↣  σ") : C_scope.
 
@@ -238,39 +238,39 @@ Ltac refine_inversion_all :=
 
 Instance memenv_refine `{Env Ti} :
     RefineM Ti (env Ti) (memenv Ti) := λ Γ f Γm1 Γm2,
-  (**i 1.) *) mem_inj_injective f ∧
+  (**i 1.) *) meminj_injective f ∧
   (**i 2.) *) (∀ o1 o2 r τ1, f !! o1 = Some (o2,r) →
     Γm1 ⊢ o1 : τ1 → ∃ τ2, Γm2 ⊢ o2 : τ2 ∧ Γ ⊢ r : τ2 ↣ τ1) ∧
   (**i 3.) *) (∀ o1 o2 r τ2, f !! o1 = Some (o2,r) →
     Γm2 ⊢ o2 : τ2 → ∃ τ1, Γm1 ⊢ o1 : τ1 ∧ Γ ⊢ r : τ2 ↣ τ1) ∧
   (**i 4.) *) (∀ o1 o2 r, f !! o1 = Some (o2,r) →
     index_alive Γm1 o1 → index_alive Γm2 o2).
-Record mem_inj_extend {Ti} (f f' : mem_inj Ti) (Γm1 Γm2 : memenv Ti) := {
-  mem_inj_extend_left o τ : Γm1 ⊢ o : τ → f' !! o = f !! o;
-  mem_inj_extend_right o o' r τ :
+Record meminj_extend {Ti} (f f' : meminj Ti) (Γm1 Γm2 : memenv Ti) := {
+  meminj_extend_left o τ : Γm1 ⊢ o : τ → f' !! o = f !! o;
+  meminj_extend_right o o' r τ :
     Γm2 ⊢ o' : τ → f' !! o = Some (o',r) → f !! o = Some (o',r)
 }.
 
 Section memenv_refine.
 Context `{EnvSpec Ti}.
-Implicit Types f : mem_inj Ti.
-Lemma memenv_refine_injective Γ f Γm1 Γm2: Γm1 ⊑{Γ,f} Γm2 → mem_inj_injective f.
+Implicit Types f : meminj Ti.
+Lemma memenv_refine_injective Γ f Γm1 Γm2: Γm1 ⊑{Γ,f} Γm2 → meminj_injective f.
 Proof. by intros [??]. Qed.
 Lemma memenv_refine_id Γ Γm : Γm ⊑{Γ} Γm.
 Proof.
   repeat split; intros; simplify_equality;
-    try setoid_rewrite ref_typed_nil; eauto using mem_inj_id_injective.
+    try setoid_rewrite ref_typed_nil; eauto using meminj_id_injective.
 Qed.
 Lemma memenv_refine_compose Γ f1 f2 Γm1 Γm2 Γm3 :
   ✓ Γ → Γm1 ⊑{Γ,f1} Γm2 → Γm2 ⊑{Γ,f2} Γm3 → Γm1 ⊑{Γ,f1 ◎ f2} Γm3.
 Proof.
   intros ? (?&?&?&?) (?&?&?&?);
-    repeat split; eauto using mem_inj_compose_injective.
-  * intros o1 o3 r τ1; rewrite lookup_mem_inj_compose_Some;
+    repeat split; eauto using meminj_compose_injective.
+  * intros o1 o3 r τ1; rewrite lookup_meminj_compose_Some;
       intros (o2&r2&r3&?&?&->) ?; setoid_rewrite ref_typed_app; naive_solver.
-  * intros o1 o3 r τ2; rewrite lookup_mem_inj_compose_Some;
+  * intros o1 o3 r τ2; rewrite lookup_meminj_compose_Some;
       intros (o2&r2&r3&?&?&->) ?; setoid_rewrite ref_typed_app; naive_solver.
-  * intros o1 o3 r; rewrite lookup_mem_inj_compose_Some; naive_solver.
+  * intros o1 o3 r; rewrite lookup_meminj_compose_Some; naive_solver.
 Qed.
 Lemma memenv_refine_weaken Γ Γ' f Γm1 Γm2 :
   ✓ Γ → Γm1 ⊑{Γ,f} Γm2 → Γ ⊆ Γ' → Γm1 ⊑{Γ',f} Γm2.
@@ -278,21 +278,21 @@ Proof.
   intros ? (?&Htyped&Htyped'&?) ?; split;
     naive_solver eauto using ref_typed_weaken.
 Qed.
-Lemma mem_inj_extend_reflexive f Γm1 Γm2 : mem_inj_extend f f Γm1 Γm2.
+Lemma meminj_extend_reflexive f Γm1 Γm2 : meminj_extend f f Γm1 Γm2.
 Proof. by split. Qed.
-Lemma mem_inj_extend_transitive f f' f'' Γm1 Γm2 Γm1' Γm2' :
-  mem_inj_extend f f' Γm1 Γm2 → mem_inj_extend f' f'' Γm1' Γm2' →
-  Γm1 ⊆{⇒} Γm1' → Γm2 ⊆{⇒} Γm2' → mem_inj_extend f f'' Γm1 Γm2.
+Lemma meminj_extend_transitive f f' f'' Γm1 Γm2 Γm1' Γm2' :
+  meminj_extend f f' Γm1 Γm2 → meminj_extend f' f'' Γm1' Γm2' →
+  Γm1 ⊆{⇒} Γm1' → Γm2 ⊆{⇒} Γm2' → meminj_extend f f'' Γm1 Γm2.
 Proof. intros [??] [??] [? _] [? _]; split; eauto using eq_trans. Qed.
-Lemma mem_inj_extend_compose f g Γm1 Γm2 :
-  mem_inj_extend mem_inj_id f Γm1 Γm1 →
-  mem_inj_extend mem_inj_id g Γm2 Γm2 → Γm1 ⊆{⇒} Γm2 →
-  mem_inj_extend mem_inj_id (g ◎ f) Γm1 Γm1.
+Lemma meminj_extend_compose f g Γm1 Γm2 :
+  meminj_extend meminj_id f Γm1 Γm1 →
+  meminj_extend meminj_id g Γm2 Γm2 → Γm1 ⊆{⇒} Γm2 →
+  meminj_extend meminj_id (g ◎ f) Γm1 Γm1.
 Proof.
   intros [Hf Hf'] [Hg Hg'] ?; split.
-  * intros o τ ?; apply lookup_mem_inj_compose_Some.
+  * intros o τ ?; apply lookup_meminj_compose_Some.
     eexists o, [], []; eauto 8 using memenv_extend_typed.
-  * intros o o'' r τ ?; rewrite lookup_mem_inj_compose_Some.
+  * intros o o'' r τ ?; rewrite lookup_meminj_compose_Some.
     intros (o'&r'&r''&Ho&Ho'&->).
     eapply Hf' in Ho'; eauto; simplify_equality.
     rewrite (right_id_L [] (++)); eauto using memenv_extend_typed.
